.

theories/Control/Worklist.v
@@ -18,24 +18,22 @@ Fixpoint schedule (next : fin_ensemble A) (seen : fset A) (todo : list A) {struc
 
 Theorem schedule_spec (next : fin_ensemble A) (seen : fset A) (todo : list A) seen' todo'
   (H_OBS : schedule next seen todo = (seen', todo'))
-  : (forall x, x ∈ seen' <-> (x ∈ seen \/ L.In x next)) /\ (forall x, L.In x todo' <-> (L.In x todo \/ (L.In x next /\ ~ x ∈ seen))) /\ (length todo' + length (FSet.data seen) = length todo + length (FSet.data seen')).
+  : (forall x, x ∈ seen' <-> (x ∈ seen \/ L.In x next)) /\ (forall x, L.In x todo' <-> (L.In x todo \/ (L.In x next /\ ~ x ∈ seen))).
 Proof.
   revert_until next. induction next as [ | v next IH]; simpl; i.
   - splits; intuition congruence.
   - des_ifs.
     + rewrite FS.mem_eq_spec in Heq.
-      find* (H_seen & H_todo & H_length) by IH.
-      splits; auto; i.
+      find* [H_seen H_todo] by IH.
+      splits; i.
       * rewrite H_seen. intuition congruence.
       * rewrite H_todo. intuition congruence.
     + rewrite FS.mem_eq_spec in Heq.
-      find* (H_seen & H_todo & H_length) by IH.
+      find* [H_seen H_todo] by IH.
       splits; i.
       * rewrite H_seen, FS.in_add_eq_iff. intuition congruence.
       * rewrite H_todo, FS.in_add_eq_iff. simpl.
         destruct (B.decide (v = x)); intuition congruence.
-      * assert (FRESH : ~ FS.In v seen) by now rewrite FS.In_eq_iff.
-        rewrite FS.length_add in H_length by exact FRESH. cbn [length] in H_length. lia.
 Qed.
 
 Lemma schedule_no_dup (next : fin_ensemble A) (seen : fset A) (todo : list A)
@@ -48,18 +46,33 @@ Proof.
   - econs; auto. rewrite FS.mem_eq_spec in Heq. ii. eauto.
 Qed.
 
+Lemma schedule_progress (next : fin_ensemble A) (seen : fset A) (todo : list A) seen' todo'
+  (H_OBS : schedule next seen todo = (seen', todo'))
+  : (seen' = seen /\ todo' = todo) \/ length (FSet.data seen) < length (FSet.data seen').
+Proof.
+  revert_until next. induction next as [ | v next IH]; simpl; i; des_ifs.
+  - left. split; congruence.
+  - eapply IH. exact H_OBS.
+  - right. rewrite FS.mem_eq_spec in Heq.
+    obtain [SEEN _] with H_OBS by schedule_spec.
+    assert (FRESH : ~ FS.In v seen) by now rewrite FS.In_eq_iff.
+    assert (INCL : incl (FSet.data (FS.add v seen)) (FSet.data seen')) by (intros y IN; rewrite SEEN; auto).
+    obtain LE with (fset_NoDup (FS.add v seen)) INCL by NoDup_incl_length.
+    rewrite FS.length_add in LE by exact FRESH. lia.
+Qed.
+
 Lemma schedule_seen (next : fin_ensemble A) (seen : fset A) (todo : list A) (x : A)
   : x ∈ fst (schedule next seen todo) <-> (x ∈ seen \/ L.In x next).
 Proof.
   destruct (schedule next seen todo) as [seen' todo'] eqn: H_OBS; simpl.
-  now obtain (? & _ & _) with H_OBS by schedule_spec.
+  now obtain [? _] with H_OBS by schedule_spec.
 Qed.
 
 Lemma schedule_pending (next : fin_ensemble A) (seen : fset A) (todo : list A) (x : A)
   : L.In x (snd (schedule next seen todo)) <-> (L.In x todo \/ (L.In x next /\ ~ x ∈ seen)).
 Proof.
   destruct (schedule next seen todo) as [seen' todo'] eqn: H_OBS; simpl.
-  now obtain (? & ? & ?) with H_OBS by schedule_spec.
+  now obtain [? ?] with H_OBS by schedule_spec.
 Qed.
 
 Variable next : A -> fin_ensemble A.
@@ -70,10 +83,10 @@ Hypothesis domain_closed : forall x, domain x -> forall y, L.In y (next x) -> do
 
 Hypothesis domain_finite : exists bound : nat, forall xs : fset A, forall INCL : forall x, x ∈ xs -> domain x, length (FSet.data xs) <= bound.
 
-Let state : Type :=
+Let State : Type :=
   fset A * list A.
 
-Definition valid (st : state) : Prop :=
+Definition valid (st : State) : Prop :=
   (forall x, x ∈ fst st -> domain x) /\ (forall x, L.In x (snd st) -> x ∈ fst st).
 
 Lemma schedule_valid (seen : fset A) (x : A) (todo : list A)
@@ -82,55 +95,45 @@ Lemma schedule_valid (seen : fset A) (x : A) (todo : list A)
 Proof.
   destruct VALID as [DOMAIN TODO]. cbn in DOMAIN, TODO.
   destruct (schedule (next x) seen todo) as [seen' todo'] eqn: H_OBS; simpl.
-  obtain (SEEN & PENDING & LENGTH) with H_OBS by schedule_spec.
+  obtain [SEEN PENDING] with H_OBS by schedule_spec.
   split; cbn; i.
   - rewrite SEEN in H. destruct H; eauto.
   - rewrite PENDING in H. rewrite SEEN. intuition eauto.
 Qed.
 
-Inductive transition : state -> state -> Prop :=
-  | transition_step (seen : fset A) (x : A) (todo : list A)
+Inductive beta : State -> State -> Prop :=
+  | beta_intro (seen : fset A) (x : A) (todo : list A)
     (VALID : valid (seen, x :: todo))
-    : transition (seen, x :: todo) (schedule (next x) seen todo).
+    : (seen, x :: todo) ~>β schedule (next x) seen todo
+  where "st ~>β st'" := (beta st st').
 
-Definition measure (bound : nat) (st : state) : nat :=
-  bound - length (FSet.data (fst st)) + length (snd st).
-
-Lemma transition_decreases (bound : nat) (st : state) (st' : state)
-  (BOUND : forall xs : fset A, forall INCL : forall x, x ∈ xs -> domain x, length (FSet.data xs) <= bound)
-  (STEP : transition st st')
-  : measure bound st' < measure bound st.
+Lemma beta_hasSN
+  : SN.hasSN beta.
 Proof.
-  inv STEP.
-  destruct (schedule (next x) seen todo) as [seen' todo'] eqn: H_OBS; simpl.
-  obtain (SEEN & PENDING & LENGTH) with H_OBS by schedule_spec.
-  obtain [DOMAIN' TODO'] with VALID by schedule_valid.
-  destruct VALID as [DOMAIN TODO]. cbn in DOMAIN, DOMAIN'.
-  obtain OLD with DOMAIN by BOUND.
-  obtain NEW with DOMAIN' by BOUND.
-  rewrite H_OBS in NEW. unfold measure. simpl in *. lia.
+  destruct domain_finite as [bound BOUND].
+  enough (SLACK : forall n : nat, forall seen : fset A, bound <= n + length (FSet.data seen) -> forall todo : list A, SN.sn beta (seen, todo)).
+  { intros [seen todo]. eapply SLACK with (n := bound). lia. }
+  induction n as [ | n IH]; intros seen ROOM todo; induction todo as [ | x todo IH_todo]; econs; intros st' STEP; inv STEP.
+  - destruct (schedule (next x) seen todo) as [seen' todo'] eqn: H_OBS.
+    obtain [[? ?] | GROW] with H_OBS by schedule_progress; intuition try congruence.
+    obtain [DOMAIN' _] with VALID by schedule_valid; rewrite H_OBS in DOMAIN'; cbn [fst] in DOMAIN'.
+    obtain LE with DOMAIN' by BOUND. lia.
+  - destruct (schedule (next x) seen todo) as [seen' todo'] eqn: H_OBS.
+    obtain [[? ?] | GROW] with H_OBS by schedule_progress; intuition try congruence.
+    obtain [DOMAIN' _] with VALID by schedule_valid; rewrite H_OBS in DOMAIN'; cbn [fst] in DOMAIN'.
+    obtain LE with DOMAIN' by BOUND. eapply IH. lia.
 Qed.
 
-Lemma transition_hasSN
-  : SN.hasSN transition.
-Proof.
-  destruct domain_finite as [bound BOUND]. intros st; pattern st; revert st.
-  eapply well_founded_induction with (R := fun st => fun st' => measure bound st < measure bound st').
-  - exact (well_founded_ltof state (measure bound)).
-  - intros st IH. econs. i. eapply IH.
-    eapply transition_decreases; eauto.
-Qed.
-
-Fixpoint run (st : state) (VALID : valid st) (NORMAL : SN.sn transition st) {struct NORMAL} : fset A.
+Fixpoint run (st : State) (VALID : valid st) (NORMAL : SN.sn beta st) {struct NORMAL} : fset A.
 Proof.
   destruct st as [seen [ | x todo]].
   - exact seen.
-  - exact (run (schedule (next x) seen todo) (schedule_valid seen x todo VALID) (SN.sn_inv (seen, x :: todo) NORMAL (schedule (next x) seen todo) (transition_step seen x todo VALID))).
+  - exact (run (schedule (next x) seen todo) (schedule_valid seen x todo VALID) (SN.sn_inv (seen, x :: todo) NORMAL (schedule (next x) seen todo) (beta_intro seen x todo VALID))).
 Defined.
 
-Fixpoint run_sound (P : A -> Prop) (st : state)
+Fixpoint run_sound (P : A -> Prop) (st : State)
   (CLOSED : forall x, P x -> forall y, L.In y (next x) -> P y)
-  (sn_st : SN.sn transition st)
+  (sn_st : SN.sn beta st)
   (H_valid : valid st)
   (INITIAL : forall x, x ∈ fst st -> P x)
   : forall x, x ∈ run st H_valid sn_st -> P x.
@@ -142,11 +145,11 @@ Proof.
     { subst st'. intros y H_y. rewrite schedule_seen in H_y. destruct H_y; eauto.
       eapply CLOSED; eauto. eapply INITIAL. eapply H_valid. cbn; auto.
     }
-    exact (run_sound P st' CLOSED (sn_st_inv st' (transition_step seen x todo H_valid)) (schedule_valid seen x todo H_valid) PRESERVED).
+    exact (run_sound P st' CLOSED (sn_st_inv st' (beta_intro seen x todo H_valid)) (schedule_valid seen x todo H_valid) PRESERVED).
 Qed.
 
-Fixpoint run_complete (st : state)
-  (sn_st : SN.sn transition st)
+Fixpoint run_complete (st : State)
+  (sn_st : SN.sn beta st)
   (VALID : valid st)
   (CLOSED : forall x, x ∈ fst st -> forall y, L.In y (next x) -> (y ∈ fst st \/ L.In x (snd st)))
   : (forall x, x ∈ fst st -> x ∈ run st VALID sn_st) /\ (forall x, forall y, x ∈ run st VALID sn_st -> L.In y (next x) -> y ∈ run st VALID sn_st).
@@ -154,7 +157,7 @@ Proof.
   destruct sn_st as [sn_st_inv]. destruct st as [seen [ | v todo]]; cbn [run].
   - split; i; auto. find* [IN | []] by CLOSED. exact IN.
   - enough (NEXT_CLOSED : forall x, x ∈ fst (schedule (next v) seen todo) -> forall y, L.In y (next x) -> (y ∈ fst (schedule (next v) seen todo) \/ L.In x (snd (schedule (next v) seen todo)))).
-    { obtain [MONOTONE CLOSED_out] with (sn_st_inv _ (transition_step seen v todo VALID)) (schedule_valid seen v todo VALID) NEXT_CLOSED by run_complete.
+    { obtain [MONOTONE CLOSED_out] with (sn_st_inv _ (beta_intro seen v todo VALID)) (schedule_valid seen v todo VALID) NEXT_CLOSED by run_complete.
       split; auto. i. eapply MONOTONE. rewrite schedule_seen. auto.
     }
     intros x IN y EDGE. rewrite schedule_seen in IN. simpl in *. destruct IN as [IN | IN].
@@ -171,7 +174,7 @@ Proof.
 Qed.
 
 Definition closure (initial : fset A) (H_initial : forall x : A, forall IN : x ∈ initial, domain x) : fset A :=
-  run (initial, FSet.data initial) (conj H_initial (fun x : A => fun IN : x ∈ initial => IN)) (SN.sn_intro_generator 64 transition_hasSN (initial, FSet.data initial)).
+  run (initial, FSet.data initial) (conj H_initial (fun x : A => fun IN : x ∈ initial => IN)) (SN.sn_intro_generator 1000 beta_hasSN (initial, FSet.data initial)).
 
 Corollary closure_sound (P : A -> Prop) (initial : fset A)
   (H_initial : forall x, x ∈ initial -> domain x)
